First take on generic definition of morph

examples/refinement/Lens.fst
@@ -11,9 +11,14 @@ open LowStar.Modifies
 open Mem_eq
 open Relations 
 
+module H = FStar.Monotonic.Heap
+module B = LowStar.Buffer
+module ST = FStar.HyperStack.ST
 module HS = FStar.HyperStack
-module H = HighComp
-module L = LowComp 
+module U32 = FStar.UInt32
+module Map = FStar.Map
+module M = LowStar.Modifies
+
 
 
 (* Standard lens class *)
@@ -25,10 +30,16 @@ class lens a b =
     put_put : x:a -> y1:b -> y2:b -> Lemma (put (put x y1) y2 == put x y2) }
 
 (* A more specific one for our case *)
-class state_lens low high = 
+class state_lens low (high:eqtype) = 
   { wf : HS.mem -> low -> Type;
+    (* pure versions *)
     to_low : h:HS.mem -> ls:low{wf h ls} -> high -> GTot (h':HS.mem{wf h' ls}); 
     to_high : HS.mem -> low -> GTot high; 
+    (* effectful versions to define morph *)         
+    to_low' : ls:low -> hs:high -> 
+              Stack unit (requires (fun h -> wf h ls)) (ensures (fun h r h' -> wf h' ls /\ to_low h ls hs == h'));
+    to_high' : ls:low -> Stack high (requires (fun h -> wf h ls)) (ensures (fun h r h' -> h == h' /\ to_high h ls = r));
+
     high_low : h:HS.mem -> ls:low{wf h ls} ->
                Lemma (to_low h ls (to_high h ls) == h);
     low_high : h:HS.mem -> ls:low{wf h ls} -> hs:high ->
@@ -37,14 +48,50 @@ class state_lens low high =
               Lemma (to_low h ls hs2 == to_low (to_low h ls hs1) ls hs2) }
 
 
-instance tuple_lens : state_lens L.lstate H.state = 
+instance tuple_lens : state_lens lstate state = 
   { wf = well_formed; 
     to_low = state_as_lstate;
     to_high = lstate_as_state;
+    to_low' = admit ();
+    to_high' = admit ();
     high_low = state_as_lstate_get_put;
     low_high = state_as_lstate_put_get;
     low_low = state_as_lstate_put_put; } 
 
+(* WPs of high computations *)
+type hwp state a = state -> (a * state -> Type) -> GTot Type
 
+let monotonic #state #a (wp:hwp state a) =
+  forall p1 p2 s. {:pattern wp s p1; wp s p2}
+    (forall x.{:pattern (p1 x) \/ (p2 x)} p1 x ==> p2 x) ==>
+    wp s p1 ==>
+    wp s p2
 
+type hwp_mon state 'a = (wp:hwp state 'a{monotonic wp})
 
+(* High compuations *)
+type high state a (wp : hwp_mon state a) = s0:state -> PURE (a * state) (wp s0)
+
+(* Low computations *)
+type low lstate hstate (#p: state_lens lstate hstate)
+         (a:Type) (wp : hwp_mon hstate a) (c : high hstate a wp) =
+         ls:lstate ->
+         Stack a
+           (requires (fun h -> wf #_ #_ #p h ls /\ (let s0 = to_high #_ #_ #p h ls in wp s0 (fun _ -> True))))
+           (ensures  (fun h r h' ->
+                       wf h' ls /\
+                      (let s0 = to_high #_ #_ #p h ls in
+                       let (x, s1) = c s0 in
+                       h' == to_low #_ #_ #p h ls s1 /\ x == r )))
+
+let run_high #hstate #a #wp (c:high hstate a wp) (s0:_{wp s0 (fun _ -> True)}) : (a * hstate) = c s0
+
+// Lifting of high programs to low programs
+let morph lstate hstate (#p: state_lens lstate hstate)
+           (a:Type) (wp : hwp_mon hstate a) (c : high hstate a wp) : low lstate hstate #p a wp c =
+  fun ls ->
+    let hs = to_high' #_ #_ #p ls in 
+    let h = ST.get () in
+    assert (to_high #_ #_ #p h ls == hs);
+    let (x, hs') = run_high c hs in
+    to_low' #_ #_ #p ls hs'; x
